Reorganize specs with cleaner names
Proofs about different specs are in their own file (CCLHoareTriples).
[cprog_ok] is the basic Hoare double, [cprog_spec] is the basic
statement using a spec but internally expressed as a double, and
[cprog_triple] is available as an actual Hoare triple interpretation
(with equivalence between [cprog_spec] and [cprog_triple].

Creates a few more files, notably separating monad laws out.

src/CCLPrimitives.v
@@ -1,136 +1,29 @@
-Require Import CCLProg.
-Require Import Eqdep.
+Require Import CCLProg CCLMonadLaws CCLHoareTriples.
 Require Import Mem Pred.
 Require Import AsyncDisk.
 Require Import Word.
 Require Import FunctionalExtensionality.
 
-Module CCLTactics.
-  Ltac inj_pair2 :=
-    match goal with
-    | [ H: existT ?P ?a _ = existT ?P ?a _ |- _ ] =>
-      apply inj_pair2 in H; subst
-    end.
-
-  Ltac inv_bind :=
-    match goal with
-    | [ H: exec _ _ _ (Bind _ _) _ |- _ ] =>
-      inversion H; subst; repeat inj_pair2;
-      try match goal with
-          | [ H: step _ _ _ _ _ |- _ ] =>
-            solve [ inversion H ]
-          | [ H: fail_step _ _ |- _ ] =>
-            solve [ inversion H ]
-          end;
-      clear H
-    end.
-
-  Ltac inv_ret :=
-    match goal with
-    | [ H: exec _ _ _ (Ret _) _ |- _ ] =>
-      inversion H; subst; repeat inj_pair2;
-      try match goal with
-          | [ H: step _ _ (Ret _) _ _ |- _ ] =>
-            solve [ inversion H ]
-          | [ H: fail_step _ (Ret _) |- _ ] =>
-            solve [ inversion H ]
-          end;
-      clear H
-    end.
-
-  Local Ltac inv_cleanup H :=
-    inversion H; subst; repeat inj_pair2.
-
-  Ltac inv_exec' H :=
-    inv_cleanup H;
-    try match goal with
-        | [ H: step _ _ _ _ _ |- _ ] => inv_cleanup H
-        | [ H: fail_step _ _ |- _ ] => inv_cleanup H
-        end; try congruence.
-
-  Ltac inv_exec :=
-    match goal with
-    | [ H: exec _ _ _ _ (Finished _ _ _) |- _ ] => inv_exec' H
-    | [ H: exec _ _ _ _ Error |- _ ] => inv_exec' H
-    end.
-
-End CCLTactics.
-
 Import CCLTactics.
 
 Section Primitives.
 
-  Variable St:StateTypes.
-  Variable G: TID -> Sigma St -> Sigma St -> Prop.
-
-  Theorem cprog_ok_weaken : forall T tid (pre pre': _ -> _ -> Prop) (p: cprog T),
-      cprog_ok G tid pre p ->
-      (forall st donecond, pre' st donecond -> pre st donecond) ->
-      cprog_ok G tid pre' p.
-  Proof.
-    intros.
-    unfold cprog_ok; intros.
-    apply H0 in H1.
-    eapply H; eauto.
-  Qed.
-
-  Definition exec_equiv T (p p': cprog T) :=
-    forall tid st out, exec G tid st p out <-> exec G tid st p' out.
-
-  Hint Constructors exec.
-
-  Theorem monad_right_id : forall T (p: cprog T),
-      exec_equiv (Bind p Ret) p.
-  Proof.
-    split; intros.
-    - inv_bind; eauto.
-      inv_ret; eauto.
-    - destruct out, st; eauto.
-  Qed.
-
-  Theorem monad_left_id : forall T T' (p: T -> cprog T') v,
-      exec_equiv (Bind (Ret v) p) (p v).
-  Proof.
-    split; intros.
-    - inv_bind.
-      inv_ret; eauto.
-      inv_ret.
-    - destruct out, st; eauto.
-  Qed.
-
-  Theorem monad_assoc : forall T T' T''
-                          (p1: cprog T)
-                          (p2: T -> cprog T')
-                          (p3: T' -> cprog T''),
-      exec_equiv (Bind (Bind p1 p2) p3) (Bind p1 (fun x => Bind (p2 x) p3)).
-  Proof.
-    split; intros;
-      repeat (inv_bind; eauto).
-  Qed.
-
-  Theorem cprog_ok_respects_exec_equiv : forall T (p p': cprog T) tid pre,
-      exec_equiv p p' ->
-      cprog_ok G tid pre p' ->
-      cprog_ok G tid pre p.
-  Proof.
-    unfold cprog_ok, exec_equiv; intros.
-    eapply H0; eauto.
-    apply H; eauto.
-  Qed.
+  Context {St:StateTypes}.
+  Variable G:Protocol St.
 
   Ltac begin_prim :=
-    unfold cprog_triple, ReflectDouble, cprog_ok; simpl; intros;
+    unfold cprog_spec, cprog_ok; simpl; intros;
     repeat deex.
 
   Theorem BeginRead_ok : forall tid a,
-      cprog_triple G tid
-                   (fun v '(sigma_i, sigma) =>
-                      {| precondition := Sigma.disk sigma a = Some (v, NoReader);
-                         postcondition :=
-                           fun '(sigma_i', sigma') _ =>
-                             sigma_i' = sigma_i /\
-                             sigma' = Sigma.upd_disk sigma (fun d => upd d a (v, Pending)); |})
-                   (BeginRead a).
+      cprog_spec G tid
+                 (fun v '(sigma_i, sigma) =>
+                    {| precondition := Sigma.disk sigma a = Some (v, NoReader);
+                       postcondition :=
+                         fun '(sigma_i', sigma') _ =>
+                           sigma_i' = sigma_i /\
+                           sigma' = Sigma.upd_disk sigma (fun d => upd d a (v, Pending)); |})
+                 (BeginRead a).
   Proof.
     begin_prim.
     inv_bind; inv_exec.
@@ -142,16 +35,16 @@ Section Primitives.
   Qed.
 
   Theorem WaitForRead_ok : forall tid a,
-      cprog_triple G tid
-                   (fun v '(sigma_i, sigma) =>
-                      {| precondition :=
-                           Sigma.disk sigma a = Some (v, Pending);
-                         postcondition :=
-                           fun '(sigma_i', sigma') r =>
-                             sigma_i' = sigma_i /\
-                             sigma' = Sigma.upd_disk sigma (fun d => upd d a (v, NoReader)) /\
-                             r = v; |})
-                   (WaitForRead a).
+      cprog_spec G tid
+                 (fun v '(sigma_i, sigma) =>
+                    {| precondition :=
+                         Sigma.disk sigma a = Some (v, Pending);
+                       postcondition :=
+                         fun '(sigma_i', sigma') r =>
+                           sigma_i' = sigma_i /\
+                           sigma' = Sigma.upd_disk sigma (fun d => upd d a (v, NoReader)) /\
+                           r = v; |})
+                 (WaitForRead a).
   Proof.
     begin_prim.
     inv_bind; inv_exec.
@@ -164,15 +57,15 @@ Section Primitives.
   Qed.
 
   Theorem Write_ok : forall tid a v,
-      cprog_triple G tid
-                   (fun v0 '(sigma_i, sigma) =>
-                      {| precondition :=
-                           Sigma.disk sigma a = Some (v0, NoReader);
-                         postcondition :=
-                           fun '(sigma_i', sigma') _ =>
-                             sigma_i' = sigma_i /\
-                             sigma' = Sigma.upd_disk sigma (fun d => upd d a (v, NoReader)); |})
-                   (Write a v).
+      cprog_spec G tid
+                 (fun v0 '(sigma_i, sigma) =>
+                    {| precondition :=
+                         Sigma.disk sigma a = Some (v0, NoReader);
+                       postcondition :=
+                         fun '(sigma_i', sigma') _ =>
+                           sigma_i' = sigma_i /\
+                           sigma' = Sigma.upd_disk sigma (fun d => upd d a (v, NoReader)); |})
+                 (Write a v).
   Proof.
     begin_prim.
     inv_bind; inv_exec.
@@ -182,15 +75,15 @@ Section Primitives.
   Qed.
 
   Theorem Get_ok : forall tid,
-      cprog_triple G tid
-                   (fun (_:unit) '(sigma_i, sigma) =>
-                      {| precondition := True;
-                         postcondition :=
-                           fun  '(sigma_i', sigma') r =>
-                             sigma_i' = sigma_i /\
-                             sigma' = sigma /\
-                             r = Sigma.mem sigma; |})
-                   Get.
+      cprog_spec G tid
+                 (fun (_:unit) '(sigma_i, sigma) =>
+                    {| precondition := True;
+                       postcondition :=
+                         fun  '(sigma_i', sigma') r =>
+                           sigma_i' = sigma_i /\
+                           sigma' = sigma /\
+                           r = Sigma.mem sigma; |})
+                 Get.
   Proof.
     begin_prim.
     inv_bind; inv_exec.
@@ -200,14 +93,14 @@ Section Primitives.
   Qed.
 
   Theorem Assgn_ok : forall tid m',
-      cprog_triple G tid
-                   (fun (_:unit) '(sigma_i, sigma) =>
-                      {| precondition := True;
-                         postcondition :=
-                           fun '(sigma_i', sigma') _ =>
-                             sigma_i' = sigma_i /\
-                             sigma' = Sigma.set_mem sigma m'; |})
-                   (Assgn m').
+      cprog_spec G tid
+                 (fun (_:unit) '(sigma_i, sigma) =>
+                    {| precondition := True;
+                       postcondition :=
+                         fun '(sigma_i', sigma') _ =>
+                           sigma_i' = sigma_i /\
+                           sigma' = Sigma.set_mem sigma m'; |})
+                 (Assgn m').
   Proof.
     begin_prim.
     inv_bind; inv_exec.
@@ -217,16 +110,16 @@ Section Primitives.
   Qed.
 
   Theorem Hash_ok : forall tid sz (buf: word sz),
-      cprog_triple G tid
-                   (fun (_:unit) '(sigma_i, sigma) =>
-                      {| precondition := True;
-                         postcondition :=
-                           fun '(sigma_i', sigma') r =>
-                             r = hash_fwd buf /\
-                             hash_safe (Sigma.hm sigma) (hash_fwd buf) buf /\
-                             sigma_i' = sigma_i /\
-                             sigma' = Sigma.upd_hm sigma buf; |})
-                   (Hash buf).
+      cprog_spec G tid
+                 (fun (_:unit) '(sigma_i, sigma) =>
+                    {| precondition := True;
+                       postcondition :=
+                         fun '(sigma_i', sigma') r =>
+                           r = hash_fwd buf /\
+                           hash_safe (Sigma.hm sigma) (hash_fwd buf) buf /\
+                           sigma_i' = sigma_i /\
+                           sigma' = Sigma.upd_hm sigma buf; |})
+                 (Hash buf).
   Proof.
     begin_prim.
     inv_bind; inv_exec.
@@ -236,15 +129,15 @@ Section Primitives.
   Qed.
 
   Theorem Ret_ok : forall tid T (v:T),
-      cprog_triple G tid
-                   (fun (_:unit) '(sigma_i, sigma) =>
-                      {| precondition := True;
-                         postcondition :=
-                           fun '(sigma_i', sigma') r =>
-                             sigma_i' = sigma_i /\
-                             sigma' = sigma /\
-                             r = v; |})
-                   (Ret v).
+      cprog_spec G tid
+                 (fun (_:unit) '(sigma_i, sigma) =>
+                    {| precondition := True;
+                       postcondition :=
+                         fun '(sigma_i', sigma') r =>
+                           sigma_i' = sigma_i /\
+                           sigma' = sigma /\
+                           r = v; |})
+                 (Ret v).
   Proof.
     begin_prim.
     inv_bind; inv_exec.
@@ -254,14 +147,14 @@ Section Primitives.
   Qed.
 
   Theorem GhostUpdate_ok : forall tid up,
-      cprog_triple G tid
-                   (fun (_:unit) '(sigma_i, sigma) =>
-                      {| precondition := True;
-                         postcondition :=
-                           fun '(sigma_i', sigma') _ =>
-                             sigma_i' = sigma_i /\
-                             sigma' = Sigma.upd_s sigma (up tid); |})
-                   (GhostUpdate up).
+      cprog_spec G tid
+                 (fun (_:unit) '(sigma_i, sigma) =>
+                    {| precondition := True;
+                       postcondition :=
+                         fun '(sigma_i', sigma') _ =>
+                           sigma_i' = sigma_i /\
+                           sigma' = Sigma.upd_s sigma (up tid); |})
+                 (GhostUpdate up).
   Proof.
     begin_prim.
     inv_bind; inv_exec.
@@ -271,14 +164,14 @@ Section Primitives.
   Qed.
 
   Theorem Yield_ok : forall tid,
-      cprog_triple G tid
-                   (fun (_:unit) '(sigma_i, sigma) =>
-                      {| precondition := G tid sigma_i sigma;
-                         postcondition :=
-                           fun '(sigma_i', sigma') _ =>
-                             Rely G tid sigma sigma' /\
-                             sigma_i' = sigma'; |})
-                   Yield.
+      cprog_spec G tid
+                 (fun (_:unit) '(sigma_i, sigma) =>
+                    {| precondition := G tid sigma_i sigma;
+                       postcondition :=
+                         fun '(sigma_i', sigma') _ =>
+                           Rely G tid sigma sigma' /\
+                           sigma_i' = sigma'; |})
+                 Yield.
   Proof.
     begin_prim.
     inv_bind; inv_exec.
