src/CCLHoareTriples.v
@@ -1,0 +1,105 @@
+Require Import CCLProg CCLMonadLaws Automation.
+
+Import CCLTactics.
+
+Section HoareTriples.
+
+  Context {St:StateTypes}.
+  Variables G:Protocol St.
+
+  Record SpecParams T :=
+    { precondition :  Prop;
+      postcondition : (Sigma St * Sigma St) ->
+                      T -> Prop }.
+
+  Definition Spec A T := A -> (Sigma St * Sigma St) -> SpecParams T.
+
+  Definition cprog_spec tid A T' (spec: Spec A T') (p: cprog T') :=
+    forall T (rx: _ -> cprog T),
+      cprog_ok G tid
+               (fun st donecond =>
+                  exists a, precondition (spec a st) /\
+                       forall r, cprog_ok G tid
+                                     (fun st' donecond_rx =>
+                                        postcondition (spec a st) st' r /\
+                                        donecond_rx = donecond) (rx r))
+               (Bind p rx).
+
+  Theorem cprog_ok_weaken : forall T tid (pre pre': _ -> _ -> Prop) (p: cprog T),
+      cprog_ok G tid pre p ->
+      (forall st donecond, pre' st donecond -> pre st donecond) ->
+      cprog_ok G tid pre' p.
+  Proof.
+    intros.
+    unfold cprog_ok; intros.
+    apply H0 in H1.
+    eapply H; eauto.
+  Qed.
+
+  (* this is really the natural interpretation of a triple, directly as a
+  correctness statement - [cprog_spec] instead unquotes triple into a double
+  (with an arbitrary continuation) and then uses the double-based correctness
+  statement *)
+  Definition cprog_triple A T tid (spec: Spec A T) (p: @cprog St T) :=
+    forall a st out,
+      precondition (spec a st) ->
+      exec G tid st p out ->
+      match out with
+      | Finished sigma_i' sigma' v => postcondition (spec a st) (sigma_i', sigma') v
+      | Error => False
+      end.
+
+  Theorem triple_spec_equiv : forall A T tid (spec: Spec A T) (p: @cprog St T),
+      cprog_spec tid spec p <->
+      cprog_triple tid spec p.
+  Proof.
+    unfold cprog_spec, cprog_triple.
+    split; intros.
+    - unfold cprog_ok at 1 in H.
+      specialize (H _ Ret st).
+      specialize (H (fun st' v => postcondition (spec a st) st' v)).
+      specialize (H out).
+
+      apply H.
+
+      exists a; intuition eauto.
+      unfold cprog_ok; intros.
+      CCLTactics.inv_ret; intuition (subst; eauto).
+
+      apply monad_right_id; auto.
+    - unfold cprog_ok at 1; intros; repeat deex.
+      CCLTactics.inv_bind.
+      match goal with
+      | [ Hexec: exec _ _ _ p _ |- _ ] =>
+        eapply H in Hexec; intuition eauto
+      end.
+      match goal with
+      | [ Hexec: exec _ _ _ (rx _) _ |- _ ] =>
+        eapply H2 in Hexec; intuition eauto
+      end.
+
+      match goal with
+      | [ Hexec: exec _ _ _ p _ |- _ ] =>
+        eapply H in Hexec; intuition eauto
+      end.
+  Qed.
+
+  Corollary spec_to_exec : forall tid A T (spec: Spec A T) a p,
+      cprog_spec tid spec p ->
+      forall st out,
+      exec G tid st p out ->
+      precondition (spec a st) ->
+      match out with
+        | Finished sigma_i' sigma' v =>
+          postcondition (spec a st) (sigma_i', sigma') v
+        | Error => False
+      end.
+  Proof.
+    intros.
+    destruct (triple_spec_equiv tid spec p); intuition.
+    match goal with
+    | [ H: cprog_triple _ _ _ |- _ ] => eapply H; eauto
+    end.
+  Qed.
+
+End HoareTriples.
