src/CCLMonadLaws.v
@@ -1,0 +1,54 @@
+Require Import CCLProg.
+
+Import CCLTactics.
+
+Section MonadLaws.
+
+  Variable St:StateTypes.
+  Variable G:Protocol St.
+
+  Definition exec_equiv T (p p': cprog T) :=
+    forall tid st out, exec G tid st p out <-> exec G tid st p' out.
+
+  Hint Constructors exec.
+
+  Theorem monad_right_id : forall T (p: cprog T),
+      exec_equiv (Bind p Ret) p.
+  Proof.
+    split; intros.
+    - inv_bind; eauto.
+      inv_ret; eauto.
+    - destruct out, st; eauto.
+  Qed.
+
+  Theorem monad_left_id : forall T T' (p: T -> cprog T') v,
+      exec_equiv (Bind (Ret v) p) (p v).
+  Proof.
+    split; intros.
+    - inv_bind.
+      inv_ret; eauto.
+      inv_ret.
+    - destruct out, st; eauto.
+  Qed.
+
+  Theorem monad_assoc : forall T T' T''
+                          (p1: cprog T)
+                          (p2: T -> cprog T')
+                          (p3: T' -> cprog T''),
+      exec_equiv (Bind (Bind p1 p2) p3) (Bind p1 (fun x => Bind (p2 x) p3)).
+  Proof.
+    split; intros;
+      repeat (inv_bind; eauto).
+  Qed.
+
+  Theorem cprog_ok_respects_exec_equiv : forall T (p p': cprog T) tid pre,
+      exec_equiv p p' ->
+      cprog_ok G tid pre p' ->
+      cprog_ok G tid pre p.
+  Proof.
+    unfold cprog_ok, exec_equiv; intros.
+    eapply H0; eauto.
+    apply H; eauto.
+  Qed.
+
+End MonadLaws.
